Kami/Ext/Extraction.v
@@ -16,10 +16,10 @@ Unset Extraction AutoInline.
 Definition rv32AddrSize := 32.
 Definition rv32IAddrSize := 10.
 
-Definition pinit: ProcInit rv32AddrSize rv32DataBytes rv32RfIdx :=
+Definition pinit: ProcInit rv32IAddrSize rv32DataBytes rv32RfIdx :=
   {| pcInit := Default; rfInit := Default |}.
 
-Definition predictNextPc ty (ppc: fullType ty (SyntaxKind (Bit rv32AddrSize))) :=
+Definition predictNextPc ty (ppc: fullType ty (SyntaxKind (Bit rv32IAddrSize))) :=
   (#ppc + $4)%kami_expr.
 
 Definition p4st: Modules :=
@@ -28,15 +28,15 @@ Definition p4st: Modules :=
     rv32GetLdDst (rv32GetLdAddr rv32AddrSize) rv32GetLdSrc (rv32CalcLdAddr rv32AddrSize)
     (rv32GetStAddr rv32AddrSize) rv32GetStSrc (rv32CalcStAddr rv32AddrSize)
     rv32GetStVSrc rv32GetSrc1 rv32GetSrc2 rv32GetDst
-    (rv32Exec rv32AddrSize) (rv32NextPc rv32AddrSize)
-    (rv32AlignPc rv32AddrSize rv32IAddrSize) (rv32AlignAddr rv32AddrSize)
+    (rv32Exec rv32IAddrSize) (rv32NextPc rv32IAddrSize)
+    (rv32AlignAddr rv32AddrSize)
     predictNextPc
-    (@d2ePackI _ _ _ _) (@d2eOpTypeI _ _ _ _) (@d2eDstI _ _ _ _) (@d2eAddrI _ _ _ _)
-    (@d2eVal1I _ _ _ _) (@d2eVal2I _ _ _ _) (@d2eRawInstI _ _ _ _) (@d2eCurPcI _ _ _ _)
-    (@d2eNextPcI _ _ _ _) (@d2eEpochI _ _ _ _)
+    (@d2ePackI _ _ _ _ _) (@d2eOpTypeI _ _ _ _ _) (@d2eDstI _ _ _ _ _) (@d2eAddrI _ _ _ _ _)
+    (@d2eVal1I _ _ _ _ _) (@d2eVal2I _ _ _ _ _) (@d2eRawInstI _ _ _ _ _) (@d2eCurPcI _ _ _ _ _)
+    (@d2eNextPcI _ _ _ _ _) (@d2eEpochI _ _ _ _ _)
     (@f2dPackI _ _) (@f2dRawInstI _ _) (@f2dCurPcI _ _)
     (@f2dNextPcI _ _) (@f2dEpochI _ _)
-    (@e2wPackI _ _ _ _) (@e2wDecInstI _ _ _ _) (@e2wValI _ _ _ _)
+    (@e2wPackI _ _ _ _ _) (@e2wDecInstI _ _ _ _ _) (@e2wValI _ _ _ _ _)
     pinit.
 
 (* targetM should be your target module *)
