Kami/Ex/ProcFourStDec.v
@@ -26,12 +26,11 @@ Section ProcFDE.
             (getSrc1: Src1T instBytes rfIdx)
             (getSrc2: Src2T instBytes rfIdx)
             (getDst: DstT instBytes rfIdx)
-            (exec: ExecT addrSize instBytes dataBytes)
-            (getNextPc: NextPcT addrSize instBytes dataBytes rfIdx)
-            (alignPc: AlignPcT addrSize iaddrSize)
+            (exec: ExecT iaddrSize instBytes dataBytes)
+            (getNextPc: NextPcT iaddrSize instBytes dataBytes rfIdx)
             (alignAddr: AlignAddrT addrSize)
-            (predictNextPc: forall ty, fullType ty (SyntaxKind (Bit addrSize)) -> (* pc *)
-                                       Expr ty (SyntaxKind (Bit addrSize))).
+            (predictNextPc: forall ty, fullType ty (SyntaxKind (Bit iaddrSize)) -> (* pc *)
+                                       Expr ty (SyntaxKind (Bit iaddrSize))).
 
   (* Abstract d2eElt *)
   Variable (d2eElt: Kind).
@@ -43,8 +42,8 @@ Section ProcFDE.
                 Expr ty (SyntaxKind (Data dataBytes)) -> (* val1 *)
                 Expr ty (SyntaxKind (Data dataBytes)) -> (* val2 *)
                 Expr ty (SyntaxKind (Data instBytes)) -> (* rawInst *)
-                Expr ty (SyntaxKind (Bit addrSize)) -> (* curPc *)
-                Expr ty (SyntaxKind (Bit addrSize)) -> (* nextPc *)
+                Expr ty (SyntaxKind (Bit iaddrSize)) -> (* curPc *)
+                Expr ty (SyntaxKind (Bit iaddrSize)) -> (* nextPc *)
                 Expr ty (SyntaxKind Bool) -> (* epoch *)
                 Expr ty (SyntaxKind d2eElt)).
   Variables
@@ -59,9 +58,9 @@ Section ProcFDE.
     (d2eRawInst: forall ty, fullType ty (SyntaxKind d2eElt) ->
                             Expr ty (SyntaxKind (Data instBytes)))
     (d2eCurPc: forall ty, fullType ty (SyntaxKind d2eElt) ->
-                          Expr ty (SyntaxKind (Bit addrSize)))
+                          Expr ty (SyntaxKind (Bit iaddrSize)))
     (d2eNextPc: forall ty, fullType ty (SyntaxKind d2eElt) ->
-                           Expr ty (SyntaxKind (Bit addrSize)))
+                           Expr ty (SyntaxKind (Bit iaddrSize)))
     (d2eEpoch: forall ty, fullType ty (SyntaxKind d2eElt) ->
                           Expr ty (SyntaxKind Bool)).
 
@@ -70,17 +69,17 @@ Section ProcFDE.
   Variable (f2dPack:
               forall ty,
                 Expr ty (SyntaxKind (Data instBytes)) -> (* rawInst *)
-                Expr ty (SyntaxKind (Bit addrSize)) -> (* curPc *)
-                Expr ty (SyntaxKind (Bit addrSize)) -> (* nextPc *)
+                Expr ty (SyntaxKind (Bit iaddrSize)) -> (* curPc *)
+                Expr ty (SyntaxKind (Bit iaddrSize)) -> (* nextPc *)
                 Expr ty (SyntaxKind Bool) -> (* epoch *)
                 Expr ty (SyntaxKind f2dElt)).
   Variables
     (f2dRawInst: forall ty, fullType ty (SyntaxKind f2dElt) ->
                             Expr ty (SyntaxKind (Data instBytes)))
     (f2dCurPc: forall ty, fullType ty (SyntaxKind f2dElt) ->
-                          Expr ty (SyntaxKind (Bit addrSize)))
+                          Expr ty (SyntaxKind (Bit iaddrSize)))
     (f2dNextPc: forall ty, fullType ty (SyntaxKind f2dElt) ->
-                           Expr ty (SyntaxKind (Bit addrSize)))
+                           Expr ty (SyntaxKind (Bit iaddrSize)))
     (f2dEpoch: forall ty, fullType ty (SyntaxKind f2dElt) ->
                           Expr ty (SyntaxKind Bool)).
 
@@ -110,12 +109,12 @@ Section ProcFDE.
     (e2wVal: forall ty, fullType ty (SyntaxKind e2wElt) ->
                         Expr ty (SyntaxKind (Data dataBytes))).
 
-  Variable (init: ProcInit addrSize dataBytes rfIdx).
+  Variable (init: ProcInit iaddrSize dataBytes rfIdx).
 
   Definition fetchDecode := ProcFetchDecode.fetchDecode
                               getOptype getLdDst getLdAddr getLdSrc calcLdAddr
                               getStAddr getStSrc calcStAddr getStVSrc
-                              getSrc1 getSrc2 getDst alignPc predictNextPc d2ePack
+                              getSrc1 getSrc2 getDst predictNextPc d2ePack
                               f2dPack f2dRawInst f2dCurPc f2dNextPc f2dEpoch
                               (pcInit init).
 
@@ -123,7 +122,7 @@ Section ProcFDE.
                         ++ regFile (rfInit init)
                         ++ scoreBoard rfIdx
                         ++ oneEltFifo d2eFifoName d2eElt
-                        ++ oneEltFifoEx1 w2dFifoName (Bit addrSize)
+                        ++ oneEltFifoEx1 w2dFifoName (Bit iaddrSize)
                         ++ (executer rfIdx exec d2eOpType d2eVal1 d2eVal2
                                      d2eRawInst d2eCurPc e2wPack)
                         ++ epoch
@@ -135,7 +134,7 @@ Section ProcFDE.
   Definition p3st := ProcThreeStage.p3st getOptype getLdDst getLdAddr getLdSrc calcLdAddr
                                          getStAddr getStSrc calcStAddr getStVSrc
                                          getSrc1 getSrc2 getDst exec getNextPc
-                                         alignPc alignAddr predictNextPc
+                                         alignAddr predictNextPc
                                          d2ePack d2eOpType d2eDst d2eAddr d2eVal1 d2eVal2
                                          d2eRawInst d2eCurPc d2eNextPc d2eEpoch
                                          e2wPack e2wDecInst e2wVal init.
