Kami/Ex/ProcThreeStDec.v
@@ -26,12 +26,11 @@ Section ProcThreeStDec.
             (getSrc1: Src1T instBytes rfIdx)
             (getSrc2: Src2T instBytes rfIdx)
             (getDst: DstT instBytes rfIdx)
-            (exec: ExecT addrSize instBytes dataBytes)
-            (getNextPc: NextPcT addrSize instBytes dataBytes rfIdx)
-            (alignPc: AlignPcT addrSize iaddrSize)
+            (exec: ExecT iaddrSize instBytes dataBytes)
+            (getNextPc: NextPcT iaddrSize instBytes dataBytes rfIdx)
             (alignAddr: AlignAddrT addrSize)
-            (predictNextPc: forall ty, fullType ty (SyntaxKind (Bit addrSize)) -> (* pc *)
-                                       Expr ty (SyntaxKind (Bit addrSize))).
+            (predictNextPc: forall ty, fullType ty (SyntaxKind (Bit iaddrSize)) -> (* pc *)
+                                       Expr ty (SyntaxKind (Bit iaddrSize))).
 
   Variable (d2eElt: Kind).
   Variable (d2ePack:
@@ -42,8 +41,8 @@ Section ProcThreeStDec.
                 Expr ty (SyntaxKind (Data dataBytes)) -> (* val1 *)
                 Expr ty (SyntaxKind (Data dataBytes)) -> (* val2 *)
                 Expr ty (SyntaxKind (Data instBytes)) -> (* rawInst *)
-                Expr ty (SyntaxKind (Bit addrSize)) -> (* curPc *)
-                Expr ty (SyntaxKind (Bit addrSize)) -> (* nextPc *)
+                Expr ty (SyntaxKind (Bit iaddrSize)) -> (* curPc *)
+                Expr ty (SyntaxKind (Bit iaddrSize)) -> (* nextPc *)
                 Expr ty (SyntaxKind Bool) -> (* epoch *)
                 Expr ty (SyntaxKind d2eElt)).
   Variables
@@ -58,9 +57,9 @@ Section ProcThreeStDec.
     (d2eRawInst: forall ty, fullType ty (SyntaxKind d2eElt) ->
                             Expr ty (SyntaxKind (Data instBytes)))
     (d2eCurPc: forall ty, fullType ty (SyntaxKind d2eElt) ->
-                          Expr ty (SyntaxKind (Bit addrSize)))
+                          Expr ty (SyntaxKind (Bit iaddrSize)))
     (d2eNextPc: forall ty, fullType ty (SyntaxKind d2eElt) ->
-                           Expr ty (SyntaxKind (Bit addrSize)))
+                           Expr ty (SyntaxKind (Bit iaddrSize)))
     (d2eEpoch: forall ty, fullType ty (SyntaxKind d2eElt) ->
                           Expr ty (SyntaxKind Bool)).
 
@@ -102,19 +101,19 @@ Section ProcThreeStDec.
     (He2wVal: forall decInst val,
         evalExpr (e2wVal _ (evalExpr (e2wPack decInst val))) = evalExpr val).
 
-  Variable (init: ProcInit addrSize dataBytes rfIdx).
+  Variable (init: ProcInit iaddrSize dataBytes rfIdx).
 
   Definition p3st := ProcThreeStage.p3st
                        getOptype getLdDst getLdAddr getLdSrc calcLdAddr
                        getStAddr getStSrc calcStAddr getStVSrc
-                       getSrc1 getSrc2 getDst exec getNextPc alignPc alignAddr predictNextPc
+                       getSrc1 getSrc2 getDst exec getNextPc alignAddr predictNextPc
                        d2ePack d2eOpType d2eDst d2eAddr d2eVal1 d2eVal2
                        d2eRawInst d2eCurPc d2eNextPc d2eEpoch
                        e2wPack e2wDecInst e2wVal init.
   Definition pdec := ProcDec.pdec
                        getOptype getLdDst getLdAddr getLdSrc calcLdAddr
                        getStAddr getStSrc calcStAddr getStVSrc
-                       getSrc1 getSrc2 getDst exec getNextPc alignPc alignAddr init.
+                       getSrc1 getSrc2 getDst exec getNextPc alignAddr init.
   
   Hint Unfold p3st: ModuleDefs. (* for kinline_compute *)
   Hint Extern 1 (ModEquiv type typeUT p3st) => unfold p3st. (* for kequiv *)
@@ -132,14 +131,14 @@ Section ProcThreeStDec.
   Hint Unfold p3st_pdec_ruleMap: MethDefs.
 
   Definition p3st_pdec_regMap (r: RegsT): RegsT :=
-    (mlet pcv : (Bit addrSize) <- r |> "pc";
+    (mlet pcv : (Bit iaddrSize) <- r |> "pc";
        mlet pgmv : (Vector (Data instBytes) iaddrSize) <- r |> "pgm";
        mlet rfv : (Vector (Data dataBytes) rfIdx) <- r |> "rf";
        mlet d2eeltv : d2eElt <- r |> "d2e"--"elt";
        mlet d2efv : Bool <- r |> "d2e"--"full";
        mlet e2weltv : e2wElt <- r |> "e2w"--"elt";
        mlet e2wfv : Bool <- r |> "e2w"--"full";
-       mlet w2deltv : Bit addrSize <- r |> "w2d"--"elt";
+       mlet w2deltv : Bit iaddrSize <- r |> "w2d"--"elt";
        mlet w2dfv : Bool <- r |> "w2d"--"full";
        mlet eev : Bool <- r |> "eEpoch";
        mlet stallv : Bool <- r |> "stall";
@@ -148,7 +147,7 @@ Section ProcThreeStDec.
        (["stall" <- existT _ _ stallv]
         +["pgm" <- existT _ _ pgmv]
         +["rf" <- existT _ _ rfv]
-        +["pc" <- existT _ (SyntaxKind (Bit addrSize))
+        +["pc" <- existT _ (SyntaxKind (Bit iaddrSize))
                (if w2dfv then w2deltv
                 else if stallv then evalExpr (d2eCurPc _ stalledv)
                      else if e2wfv then
@@ -220,7 +219,7 @@ Section ProcThreeStDec.
   Definition p3stInl := ProcThreeStInl.p3stInl getOptype getLdDst getLdAddr getLdSrc calcLdAddr
                                                getStAddr getStSrc calcStAddr getStVSrc
                                                getSrc1 getSrc2 getDst exec
-                                               getNextPc alignPc alignAddr predictNextPc
+                                               getNextPc alignAddr predictNextPc
                                                d2ePack d2eOpType d2eDst d2eAddr d2eVal1 d2eVal2
                                                d2eRawInst d2eCurPc d2eNextPc d2eEpoch
                                                e2wPack e2wDecInst e2wVal init.
